Flapjack/Test/Backend.lean
@@ -12,6 +12,7 @@ import Flapjack.Test.AllocatorRegAlloc
 import Flapjack.Test.MustTerminate
 import Flapjack.Test.TailCalls
 import Flapjack.Test.WordOperations
+import Flapjack.Test.WordBitmaps
 import Flapjack.Test.WordToStack
 import Flapjack.Test.ParallelMove
 import Flapjack.Test.Stack
